remove ops

SSASlow.lean
@@ -33,25 +33,19 @@ def Var.unit : Var := { name := "_", kind := .unit }
 -- Tag for variants of Op/Region hybrid
 inductive OR: Type
 | O -- Single Op
-| Os -- Multiple Ops
 
 -- Tagged expressiontrees
 inductive Expr: OR -> Type where
-| opsone: Expr .O -> Expr .Os -- terminator in a sequence of Ops
-| opscons: Expr .O -> Expr .Os -> Expr .Os -- cons cell 'op :: ops'
 | op (ret : Var)
    (name : String)
    (arg : List Var): Expr .O -- '%ret:retty = 'name'(%var:varty) [regions*] {const}'
 
 abbrev Op := Expr .O
-abbrev Ops := Expr .Os
 
 def Op.mk (ret: Var := Var.unit)
   (name: String)
   (arg: Var := Var.unit) : Op := Expr.op ret name [arg]
 
-def Op.Ret : Op → Var
-| .op ret _ _ => ret 
 
 -- Lean type that corresponds to kind.
 @[reducible, simp]
@@ -95,24 +89,6 @@ inductive Env where
 | empty: Env
 | cons (var: Var) (val: var.kind.eval) (rest: Env): Env 
 
-inductive OpM (a: Type) where 
-| Ret: a →OpM a
-| Get: Var → (NamedVal → OpM a) → OpM a
-| Set: (v: NamedVal) → (rest: OpM a) → OpM a   
--- | RunRegion: (List Val → OpM a) → OpM a
-| Error: String → OpM a 
-
-def OpM.bind: OpM α → (α → OpM β) → OpM β
-| .Ret a, f => f a
-| .Error s, _f => .Error s
-| .Get v k, f => .Get v (fun w => (k w).bind f)
-| .Set v rest, f => .Set v (rest.bind f)
--- | .RunRegion g args, f=> .RunRegion (fun a => (g a).bind f) args
-
-instance : Monad OpM where
-  pure := .Ret
-  bind := OpM.bind
-
 abbrev ErrorKind := String
 abbrev TopM (α : Type) : Type := StateT Env (Except ErrorKind) α
 
@@ -130,7 +106,6 @@ def Env.get (var: Var): Env → Except ErrorKind NamedVal
 def TopM.get (var: Var): TopM NamedVal := do 
   let e ← StateT.get 
   Env.get var e
-def OpM.get (var: Var): OpM NamedVal := OpM.Get var pure
 
 def TopM.set (nv: NamedVal)  (k: TopM α): TopM α := do 
   let e ← StateT.get
@@ -139,26 +114,8 @@ def TopM.set (nv: NamedVal)  (k: TopM α): TopM α := do
   let out ← k
   StateT.set e 
   return out 
-def OpM.set (nv: NamedVal)  (k: OpM α): OpM α := OpM.Set nv k
-def OpM.set' (nv: NamedVal) : OpM Unit := OpM.Set nv (pure ())
 
 def TopM.error (e: ErrorKind) : TopM α := Except.error e
-def OpM.error (e: ErrorKind): OpM α := OpM.Error e
-
-def OpM.toTopM: OpM a → TopM a
-| OpM.Ret a => return a
-| OpM.Error e => TopM.error e
-| OpM.Get var k => do 
-    let out ← TopM.get var
-    (k out).toTopM 
-| OpM.Set nv rest => do
-   TopM.set nv (rest.toTopM)
--- | OpM.RunRegion k args =>  (k args).toTopM
-
-def Val.cast (val: Val) (t: Kind): OpM t.eval :=
-  if H : val.kind = t
-  then pure (H ▸ val.val)
-  else OpM.error s!"mismatched type "
 
 -- Runtime denotation of an Op, that has evaluated its arguments,
 -- and expects a return value of type ⟦retkind⟧ 
@@ -167,37 +124,25 @@ inductive Op' where
   (name : String)
   (argval : List Val)
 
-def Op'.name: Op' → String 
-| .mk name argval => name 
-
-def Op'.argval: Op' → List Val 
-| .mk name argval => argval
-
-
 @[reducible]
 def AST.OR.denoteType: OR -> Type
-| .O => OpM NamedVal
-| .Os => OpM NamedVal
+| .O => TopM NamedVal
 
 def AST.Expr.denote {kind: OR}
- (sem: (o: Op') → OpM Val): Expr kind → kind.denoteType 
-| .opsone o => AST.Expr.denote (kind := .O) sem o
-| .opscons o os => do
-    let retv ← AST.Expr.denote (kind := .O) sem o
-    OpM.set retv (os.denote sem)
+ (sem: (o: Op') → TopM Val): Expr kind → kind.denoteType 
 | .op ret name args  => do 
-    let vals ← args.mapM OpM.get
+    let vals ← args.mapM TopM.get
     let op' : Op' := .mk
       name
       (vals.map NamedVal.toVal)
     let out ← sem op'
     if ret.kind = out.kind
     then return { name := ret.name,  kind := out.kind, val := out.val : NamedVal }
-    else OpM.error "unexpected return kind '{}', expected {}"
+    else TopM.error "unexpected return kind '{}', expected {}"
 
-def runOps (sem : (o: Op') → OpM Val) (expr: AST.Expr .Os)
+def runOp (sem : (o: Op') → TopM Val) (expr: AST.Expr .O)
 (env :  Env := Env.empty) : Except ErrorKind (NamedVal × Env) := 
-  (expr.denote sem).toTopM.run env
+  (expr.denote sem).run env
 
 
 end Semantics
@@ -205,8 +150,8 @@ end Semantics
 namespace Arith
 
 set_option pp.all true in 
-def sem: (o: Op') → OpM Val
-| .mk "float" [] => return ⟨.float, x+1⟩
+def sem: (o: Op') → TopM Val
+| .mk "float" [⟨.float, x⟩] => return ⟨.float, x+1⟩
 | .mk "float2" [⟨.float, x⟩] => return ⟨.float, x + x⟩
 | .mk "int2" [⟨.int, x⟩] => return ⟨.int, x + x⟩
 | .mk "nat2" [⟨.nat, x⟩] => return ⟨.nat, x + x⟩
@@ -221,17 +166,11 @@ def sem: (o: Op') → OpM Val
     let i := t 0 0
     let j := t 1 1
     return ⟨.int, i + i⟩
-| op => OpM.error s!"unknown op"
+| op => TopM.error s!"unknown op"
 
 
 open AST in 
-def eg_region_sub : Ops := 
-  .opsone (Op.mk (name := "float") )
-#reduce eg_region_sub
-
-open AST in 
-theorem Fail: runOps sem eg_region_sub   = .ok output  := by {
-  simp[eg_region_sub];
+theorem Fail: runOp sem  (Op.mk (name := "float"))   = .ok output  := by {
   -- ERROR:
   -- tactic 'simp' failed, nested error:
   -- (deterministic) timeout at 'whnf', maximum number of heartbeats (200000) has been reached (use 'set_option maxHeartbeats <num>' to set the limit)
